@prefix ceds: <http://ceds.ed.gov/terms#> .
@prefix cepi: <http://cepi-dev.state.mi.us/> .
@prefix dc: <http://purl.org/dc/elements/1.1/> .
@prefix owl: <http://www.w3.org/2002/07/owl#> .
@prefix rdf: <http://www.w3.org/1999/02/22-rdf-syntax-ns#> .
@prefix rdfs: <http://www.w3.org/2000/01/rdf-schema#> .
@prefix schema: <https://schema.org/> .
@prefix skos: <http://www.w3.org/2004/02/skos/core#> .

ceds:P001917 schema:domainIncludes ceds:C200411 .

ceds:P001918 schema:domainIncludes ceds:C200411 .

cepi:NI000603100001 a ceds:C000603,
        owl:NamedIndividual,
        skos:Concept ;
    rdfs:label "Count Day" ;
    dc:creator "Center for Educational Performance and Information" ;
    dc:description "The official day when data is scheduled to be counted; the data is counted as of this day." ;
    dc:identifier "cepi:NI000603100001" ;
    skos:definition "The official day when data is scheduled to be counted; the data is counted as of this day." ;
    skos:inScheme ceds:C000603 ;
    skos:notation "CountDay" ;
    skos:prefLabel "Count Day" .

cepi:NI001301000001 a ceds:C002175,
        owl:NamedIndividual,
        skos:Concept ;
    rdfs:label "Developmental Kindergarten" ;
    dc:creator "Center for Educational Performance and Information" ;
    dc:description "Developmental Kindergarten is a grade offered by the education institution.  It is the first year of a defined two-year kindergarten program that precedes entry into first grade." ;
    dc:identifier "cepi:NI001301000001" ;
    skos:definition "Developmental Kindergarten is a grade offered by the education institution.  It is the first year of a defined two-year kindergarten program that precedes entry into first grade." ;
    skos:inScheme ceds:C002175 ;
    skos:notation "DK" ;
    skos:prefLabel "Developmental Kindergarten" .

cepi:P000001 a rdf:Property ;
    rdfs:label "Data Corrections End Date " ;
    dc:creator "Center for Educational Performance and Information" ;
    dc:description "The latest date (YYYY-MM-DD) that data  were allowed to be corrected." ;
    dc:identifier "cepi:P000001" ;
    rdfs:comment "The latest date (YYYY-MM-DD) that data  were allowed to be corrected." ;
    skos:notation "DataCorrectionsEndDate" ;
    skos:prefLabel "Data Corrections End Date " ;
    schema:domainIncludes ceds:C200410 .

cepi:P000006 a rdf:Property ;
    rdfs:label "Data Collection Certification Open Date" ;
    dc:creator "Center for Educational Performance and Information" ;
    dc:description "The date and time the window for certifying a data collection opens or commences." ;
    dc:identifier "cepi:P000006" ;
    rdfs:comment "The date and time the window for certifying a data collection opens or commences." ;
    skos:notation "DataCollectionCertificationOpenDate" ;
    skos:prefLabel "Data Collection Certification Open Date" ;
    schema:domainIncludes ceds:C200410 .

cepi:P000007 a rdf:Property ;
    rdfs:label "Data Collection Certification Close Date" ;
    dc:creator "Center for Educational Performance and Information" ;
    dc:description "The date and time the window for certifying a data collection closes or ends." ;
    dc:identifier "cepi:P000007" ;
    rdfs:comment "The date and time the window for certifying a data collection closes or ends." ;
    skos:notation "DataCollectionCertificationCloseDate" ;
    skos:prefLabel "Data Collection Certification Close Date" ;
    schema:domainIncludes ceds:C200410 .

cepi:P200072 a rdf:Property ;
    rdfs:label "Grade Level Range Title" ;
    dc:creator "Center for Educational Performance and Information" ;
    dc:description "The title or name given to refer to a specific grade and/or grade range." ;
    dc:identifier "cepi:P200072" ;
    rdfs:comment "The title or name given to refer to a specific grade and/or grade range." ;
    skos:notation "GradeLevelRangeTitle" ;
    skos:prefLabel "Grade Level Range Title" ;
    schema:domainIncludes ceds:C200418 .

