@prefix ceds: <http://ceds.ed.gov/terms#> .
@prefix cepi: <http://cepi-dev.state.mi.us/> .
@prefix dc: <http://purl.org/dc/elements/1.1/> .
@prefix owl: <http://www.w3.org/2002/07/owl#> .
@prefix rdf: <http://www.w3.org/1999/02/22-rdf-syntax-ns#> .
@prefix rdfs: <http://www.w3.org/2000/01/rdf-schema#> .
@prefix schema: <https://schema.org/> .
@prefix skos: <http://www.w3.org/2004/02/skos/core#> .

ceds:P000141 schema:domainIncludes cepi:C000009.

cepi:C000009 a rdfs:Class ;
    rdfs:label "Highest Level Of Education Completed Detail" ;
    dc:creator "Center for Educational Performance and Information" ;
    dc:identifier "cepi:C000009" ;
    rdfs:comment "Details reported about the extent of formal instruction a person has received (e.g., the highest grade in school completed or its equivalent or the highest degree received) as reported by LEAs." ;
    rdfs:subClassOf ceds:C000000 ;
    skos:definition "Details reported about the extent of formal instruction a person has received (e.g., the highest grade in school completed or its equivalent or the highest degree received) as reported by LEAs." ;
    skos:notation "HighestLevelOfEducationCompletedDetail" ;
    skos:prefLabel "Highest Level Of Education Completed Detail" .

cepi:P000118 a rdf:Property ;
    rdfs:label "has Highest Level Of Education Completed Detail " ;
    dc:creator "Center for Educational Performance and Information" ;
    dc:description "Details reported about the extent of formal instruction a person has received (e.g., the highest grade in school completed or its equivalent or the highest degree received) as reported by LEAs." ;
    dc:identifier "cepi:P000118" ;
    rdfs:comment "Details reported about the extent of formal instruction a person has received (e.g., the highest grade in school completed or its equivalent or the highest degree received) as reported by LEAs." ;
    skos:notation "hasHighestLevelOfEducationCompletedDetail" ;
    skos:prefLabel "has Highest Level Of Education Completed Detail " ;
    schema:domainIncludes ceds:C200275 ;
    schema:rangeIncludes cepi:C000009 .

cepi:NI001571100001 a ceds:C001571,
        owl:NamedIndividual,
        skos:Concept ;
    rdfs:label "MOECS generated system key for a unique educator" ;
    dc:creator "Center for Educational Performance and Information" ;
    dc:description "This Staff Identifier is assigned by MOECS as a system key." ;
    dc:identifier "cepi:NI001571100001" ;
    skos:definition "This Staff Identifier is assigned by MOECS as a system key." ;
    skos:inScheme ceds:C001571 ;
    skos:notation "EducatorID" ;
    skos:prefLabel "MOECS generated system key for a unique educator" .

cepi:NI000141100001 a ceds:C000141,
        owl:NamedIndividual,
        skos:Concept ;
    rdfs:label "Medical Degree" ;
    dc:creator "Center for Educational Performance and Information" ;
    dc:description "This is a legacy option from REP that indicates the person has a postsecondary degree related to medicine but the level of the degree is unknown." ;
    dc:identifier "cepi:NI000141100001" ;
    skos:definition "This is a legacy option from REP that indicates the person has a postsecondary degree related to medicine but the level of the degree is unknown." ;
    skos:inScheme ceds:C000141 ;
    skos:notation "MedicalDegree" ;
    skos:prefLabel "Medical Degree" .
